code/hash/Hacl.Hash.Blake2.fsti
@@ -17,15 +17,15 @@ open Hacl.Hash.Definitions
 
 include Hacl.Hash.Core.Blake2
 
-val update_multi_blake2s_32: update_multi_st Blake2S Blake2.M32
-val update_multi_blake2s_128: update_multi_st Blake2S Blake2.M128
-val update_multi_blake2b_32: update_multi_st Blake2B Blake2.M32
-val update_multi_blake2b_256: update_multi_st Blake2B Blake2.M256
+val update_multi_blake2s_32: update_multi_st (|Blake2S, Blake2.M32|)
+val update_multi_blake2s_128: update_multi_st (|Blake2S, Blake2.M128|)
+val update_multi_blake2b_32: update_multi_st (|Blake2B, Blake2.M32|)
+val update_multi_blake2b_256: update_multi_st (|Blake2B, Blake2.M256|)
 
-val update_last_blake2s_32: update_last_st Blake2S Blake2.M32
-val update_last_blake2s_128: update_last_st Blake2S Blake2.M128
-val update_last_blake2b_32: update_last_st Blake2B Blake2.M32
-val update_last_blake2b_256: update_last_st Blake2B Blake2.M256
+val update_last_blake2s_32: update_last_st (|Blake2S, Blake2.M32|)
+val update_last_blake2s_128: update_last_st (|Blake2S, Blake2.M128|)
+val update_last_blake2b_32: update_last_st (|Blake2B, Blake2.M32|)
+val update_last_blake2b_256: update_last_st (|Blake2B, Blake2.M256|)
 
 val hash_blake2s_32: hash_st Blake2S
 val hash_blake2s_128: hash_st Blake2S
