code/hash/Hacl.Hash.Core.SHA1.fsti
@@ -4,8 +4,8 @@ open Hacl.Hash.Definitions
 open Spec.Hash.Definitions
 
 noextract inline_for_extraction
-val legacy_alloca: alloca_st SHA1 ()
-val legacy_init: init_st SHA1 ()
-val legacy_update: update_st SHA1 ()
+val legacy_alloca: alloca_st (|SHA1, ()|)
+val legacy_init: init_st (|SHA1, ()|)
+val legacy_update: update_st (|SHA1, ()|)
 val legacy_pad: pad_st SHA1
-val legacy_finish: finish_st SHA1 ()
+val legacy_finish: finish_st (|SHA1, ()|)
